Refactoring of the object type.

LambdaS5/caml/PrettyPrint.ml
@@ -36,10 +36,10 @@ and string_of_object_ptr depth st ptr =
     | Some obj -> string_of_object (depth-1) st obj
 and string_of_object depth st obj =
   Printf.sprintf "{[#proto: %s, #class: %s, #extensible: %B, #primval: %s, #code: %s] %s}"
-  (string_of_value depth st obj.object_proto) (String.of_list obj.object_class)
-  (obj.object_extensible) (string_of_value depth st obj.object_prim_value)
-  (string_of_value depth st obj.object_code)
-  (string_of_prop_list depth st (HeapUtils.Heap.to_list obj.object_properties_) [])
+  (string_of_value depth st (object_proto obj)) (String.of_list (object_class obj))
+  (object_extensible obj) (string_of_value depth st (object_prim_value obj))
+  (string_of_value depth st (object_code obj))
+  (string_of_prop_list depth st (HeapUtils.Heap.to_list (object_properties obj)) [])
 and string_of_prop_list depth st l skip =
   let string_of_prop = function (name, attr) ->
     Printf.sprintf "'%s': %s" (String.of_list name) (string_of_attr depth st attr)
